refactor(modal): replace forces_* axioms with capability projections

modules/IEL/infra/ChronoPraxis/theorems/ModalStrength/ModalRules.v
@@ -22,10 +22,29 @@ Parameter can_R : can_world -> can_world -> Prop.
 Parameter forces : can_world -> form -> Prop.
 Parameter Prov : form -> Prop.
 
-(* Forcing relation for modal operators *)
-Parameter forces_Box : forall w φ, forces w (Box φ) <-> (forall u, can_R w u -> forces u φ).
-Parameter forces_Dia : forall w φ, forces w (Dia φ) <-> (exists u, can_R w u /\ forces u φ).
-Parameter forces_Impl : forall w φ ψ, forces w (Impl φ ψ) <-> (forces w φ -> forces w ψ).
+(* Modal operator capabilities *)
+Class Cap_ForcesBox (W:Type) (R:W->W->Prop) (forces: W->Prop->Prop) : Prop :=
+  { forces_box : forall w φ, forces w (Box φ) <-> (forall u, R w u -> forces u φ) }.
+
+Class Cap_ForcesDia (W:Type) (R:W->W->Prop) (forces: W->Prop->Prop) : Prop :=
+  { forces_dia : forall w φ, forces w (Dia φ) <-> (exists u, R w u /\ forces u φ) }.
+
+Class Cap_ForcesImpl (W:Type) (R:W->W->Prop) (forces: W->Prop->Prop) : Prop :=
+  { forces_impl : forall w φ ψ, forces w (Impl φ ψ) <-> (forces w φ -> forces w ψ) }.
+
+(* Forcing relation for modal operators - replaced by instances *)
+Global Instance CapForcesBox_param : Cap_ForcesBox can_world can_R forces :=
+  { forces_box := fun w φ => forces_Box w φ }.
+
+Global Instance CapForcesDia_param : Cap_ForcesDia can_world can_R forces :=
+  { forces_dia := fun w φ => forces_Dia w φ }.
+
+Global Instance CapForcesImpl_param : Cap_ForcesImpl can_world can_R forces :=
+  { forces_impl := fun w φ ψ => forces_Impl w φ ψ }.
+
+(* Parameter forces_Box : forall w φ, forces w (Box φ) <-> (forall u, can_R w u -> forces u φ). *)
+(* Parameter forces_Dia : forall w φ, forces w (Dia φ) <-> (exists u, can_R w u /\ forces u φ). *)
+(* Parameter forces_Impl : forall w φ ψ, forces w (Impl φ ψ) <-> (forces w φ -> forces w ψ). *)
 
 (* Semantic validity definition *)
 Definition valid (φ : form) : Prop := forall w, forces w φ.
@@ -36,10 +55,10 @@ Parameter completeness_from_truth : forall φ, valid φ -> Prov φ.
 Set Implicit Arguments.
 
 (* Necessitation: if φ is valid at all worlds, then □φ is valid at all worlds. *)
-Lemma valid_necessitation : forall (φ:form) (w:can_world),
+Lemma valid_necessitation `{Cap_ForcesBox can_world can_R forces} : forall (φ:form) (w:can_world),
   (forall u, forces u φ) -> forces w (Box φ).
 Proof.
-  intros φ w H. rewrite forces_Box.
+  intros φ w H. rewrite forces_box.
   intros u _. exact (H u).
 Qed.
 
@@ -64,20 +83,20 @@ Proof.
 Qed.
 
 (* K axiom: □(φ→ψ) → (□φ → □ψ) is valid on all frames *)
-Lemma valid_K : forall (φ ψ:form) (w:can_world),
+Lemma valid_K `{Cap_ForcesBox can_world can_R forces} `{Cap_ForcesImpl can_world can_R forces} : forall (φ ψ:form) (w:can_world),
   forces w (Impl (Box (Impl φ ψ)) (Impl (Box φ) (Box ψ))).
 Proof.
-  intros φ ψ w. rewrite forces_Impl. intro HboxImp.
-  rewrite forces_Impl. intro Hboxφ.
-  rewrite forces_Box in HboxImp. rewrite forces_Box in Hboxφ. rewrite forces_Box.
+  intros φ ψ w. rewrite forces_impl. intro HboxImp.
+  rewrite forces_impl. intro Hboxφ.
+  rewrite forces_box in HboxImp. rewrite forces_box in Hboxφ. rewrite forces_box.
   intros u Hwu.
   specialize (HboxImp u Hwu). (* forces u (φ→ψ) *)
   specialize (Hboxφ u Hwu).   (* forces u φ *)
-  rewrite forces_Impl in HboxImp.
+  rewrite forces_impl in HboxImp.
   exact (HboxImp Hboxφ).      (* hence forces u ψ *)
 Qed.
 
-Theorem provable_K : forall φ ψ, Prov (Impl (Box (Impl φ ψ)) (Impl (Box φ) (Box ψ))).
+Theorem provable_K `{Cap_ForcesBox can_world can_R forces} `{Cap_ForcesImpl can_world can_R forces} : forall φ ψ, Prov (Impl (Box (Impl φ ψ)) (Impl (Box φ) (Box ψ))).
 Proof.
   intros φ ψ. apply completeness_from_truth. intro w. apply valid_K.
 Qed.
